- add sig and ott for fsub - change ftyp, fexp to typ, exp

fsub/autosubst2/language.sig
@@ -1,13 +1,17 @@
 -- the types
 typ : Type
 exp : Type
+entry : Type
 
 -- the constructors for typ
 typ_arr : typ -> typ -> typ
-typ_all : (bind typ in typ) -> typ
+typ_all : typ -> (bind typ in typ) -> typ
 
 -- the constructors for exp
 exp_app  : exp -> exp -> exp
 exp_abs  : typ -> (bind exp in exp) -> exp
 exp_tapp : exp -> typ -> exp
 exp_tabs : (bind typ in exp) -> exp
+
+entry_var : typ -> entry
+entry_tvar : typ -> entry
