systemf/lngen/typing.v
@@ -4,29 +4,29 @@ Require Import systemf.lngen.prop_ln.
 
 Inductive ctx_entry :=
 | tvar
-| var_typ (A : ftyp).
+| var_typ (A : typ).
 
 Definition ctx := list (atom * ctx_entry).
 
 Reserved Notation "Γ ⊢ t : A" 
   (at level 50, t at next level, no associativity).
-Inductive typing : ctx -> fexp -> ftyp -> Prop :=
-| typing_var : forall (Γ : ctx) (x : atom) (A : ftyp),
+Inductive typing : ctx -> exp -> typ -> Prop :=
+| typing_var : forall (Γ : ctx) (x : atom) (A : typ),
   binds x (var_typ A) Γ ->
-  Γ ⊢ (fexp_var_f x) : A
-| typing_abs : forall (L : atoms) (Γ : ctx) (A B : ftyp) (t : fexp),
+  Γ ⊢ (exp_var_f x) : A
+| typing_abs : forall (L : atoms) (Γ : ctx) (A B : typ) (t : exp),
   (forall x, 
     x `notin` L -> ((x , var_typ A) :: Γ) ⊢ t : B) ->
-  Γ ⊢ (fexp_abs A t) : (ftyp_arr A B)
-| typing_app : forall (Γ : ctx) (s t : fexp) (A B : ftyp),
-  Γ ⊢ s : (ftyp_arr A B) ->
+  Γ ⊢ (exp_abs A t) : (typ_arr A B)
+| typing_app : forall (Γ : ctx) (s t : exp) (A B : typ),
+  Γ ⊢ s : (typ_arr A B) ->
   Γ ⊢ t : A ->
-  Γ ⊢ (fexp_app s t) : B
-| typing_tabs : forall (L : atoms) (Γ : ctx) (t : fexp) (A : ftyp),
+  Γ ⊢ (exp_app s t) : B
+| typing_tabs : forall (L : atoms) (Γ : ctx) (t : exp) (A : typ),
   (forall X, X `notin` L -> 
-    ((X , tvar) :: Γ) ⊢ t : open_ftyp_wrt_ftyp A (ftyp_var_f X)) ->
-  Γ ⊢ (fexp_tabs t) : (ftyp_all A)
-| typing_tapp : forall (Γ : ctx) (t : fexp) (A B A' : ftyp),
-  Γ ⊢ t : (ftyp_all A) ->
-  Γ ⊢ fexp_tapp t B : (open_ftyp_wrt_ftyp A B)
+    ((X , tvar) :: Γ) ⊢ t : open_typ_wrt_typ A (typ_var_f X)) ->
+  Γ ⊢ (exp_tabs t) : (typ_all A)
+| typing_tapp : forall (Γ : ctx) (t : exp) (A B A' : typ),
+  Γ ⊢ t : (typ_all A) ->
+  Γ ⊢ exp_tapp t B : (open_typ_wrt_typ A B)
 where "Γ ⊢ t : A" := (typing Γ t A).
