stlc/autosubst2/def_typing.v
@@ -1,1 +1,3 @@
 Require Import stlc.autosubst2.def.
+
+(* https://github.com/yiyunliu/autosubst-stlc/blob/master/typing.v *)
